shiftreset/Examples.v
@@ -52,6 +52,7 @@ Proof.
   apply ent_defun_left.
   {
     apply weaken_seq.
+    unfold can_weaken_env.
     admit.
     admit.
   (* unfold can_weaken_env.
